reflection v2: remove ident hack

ocaml/fstar-lib/FStar_Reflection_Types.ml
@@ -16,8 +16,7 @@ type universe_uvar = FStar_Syntax_Syntax.universe_uvar
 type universe = FStar_Syntax_Syntax.universe
 
 type name        = string list
-type __ident     = FStar_Ident.ident
-type ident       = string * FStar_Compiler_Range.range
+type ident       = FStar_Ident.ident
 type univ_name   = ident
 type typ         = term
 type binders     = binder list
