src/reflection/FStar.Reflection.V1.Embeddings.fst
@@ -98,12 +98,8 @@ let e_aqualv =
     in
     mk_emb embed_aqualv unembed_aqualv  fstar_refl_aqualv
 
-let e_ident : embedding I.ident =
-    let repr = e_tuple2 e_string e_range in
-    embed_as repr
-             I.mk_ident
-             (fun i -> I.string_of_id i, I.range_of_id i)
-             (Some fstar_refl_ident)
+let e_ident : embedding RD.ident =
+    e_tuple2 e_string e_range
 
 let e_universe_view =
   let embed_universe_view (rng:Range.range) (uv:universe_view) : term =
