src/reflection/FStar.Reflection.V2.NBEEmbeddings.fsti
@@ -55,10 +55,9 @@ val e_attribute     : embedding attribute
 val e_attributes    : embedding (list attribute) (* This seems rather silly, but `attributes` is a keyword *)
 val e_qualifier     : embedding RD.qualifier
 val e_qualifiers    : embedding (list RD.qualifier)
-val e_ident         : embedding Ident.ident (* fake *)
-val e___ident       : embedding Ident.ident (* real *)
-val e_univ_name     : embedding (string & Range.range)
-val e_univ_names    : embedding (list (string & Range.range))
+val e_ident         : embedding Ident.ident
+val e_univ_name     : embedding univ_name
+val e_univ_names    : embedding (list univ_name)
 val e_universe      : embedding universe
 val e_universe_view : embedding universe_view
 val e_subst_elt     : embedding subst_elt
