ulib/FStar.Reflection.V2.TermEq.fst
@@ -189,8 +189,12 @@ let range_cmp r1 r2 =
 
 val ident_cmp : comparator_for ident
 let ident_cmp i1 i2 =
-  Sealed.sealed_singl (snd i1) (snd i2);
-  eq_cmp (fst i1) (fst i2)
+  let iv1 = inspect_ident i1 in
+  let iv2 = inspect_ident i2 in
+  pack_inspect_ident i1;
+  pack_inspect_ident i2;
+  Sealed.sealed_singl (snd iv1) (snd iv2);
+  eq_cmp (fst iv1) (fst iv2)
 
 val univ_cmp : comparator_for universe
 let rec univ_cmp (u1 u2 : universe) =
